stableness going away

red-black.dfy
@@ -56,7 +56,7 @@ predicate ValueIsOrdered(value: int, side: Side, pivot: int)
     if side.Left? then value <= pivot else value >= pivot
 }
 
-// The not-recursive that the set of elements on the left (resp) is on
+// The not-recursive property that the set of elements on the left (resp) is on
 // the correct side of the pivot.
 predicate SideIsOrdered(subtree: Node, side: Side, pivot: int)
 {
@@ -112,65 +112,42 @@ function method opposite(side: Side) : Side
 
 datatype Option<T> = None | Some(t: T)
 
-method RotateRight(a: Node, ghost kc: int) returns (b: Node)
-    requires RBTree(a, kc);
-    requires !a.Nil? && !a.left.Nil?;
-    ensures !b.Nil?;
-    ensures Contents(a) == Contents(b);
-{
-    var l := a.left;
-    var r := Node(l.right, a.value, a.right, Black);
-
-    // Dafny needs help realizing why everything in r is right of l.value;
-    // it needs me to point out that l.value < a.value.
-    forall x | x in Contents(r) 
-        ensures l.value <= x;
-    {
-        assert OrderedTree(l);
-        assert l.value in Contents(a.left);
-        // Think about the cases, Dafny! (In particular, expand Contents).
-        if x in Contents(r.left) {
-        } else if x in Contents(r.right) {
-        } else if x in multiset{r.value} {
-        }
-    }
-    // A similar property that r.left (l.right) is left of r.value, because
-    // it was left of a.value in the precondition.
-    forall x | x in Contents(r.left)
-        ensures x <= r.value;
-    {
-        assert x in Contents(a.left);
-    }
-
-    b := Node(l.left, l.value, r, Black);
-}
-
-method RotateLeft(a: Node, ghost kc: int) returns (b: Node)
-    requires RBTree(a, kc);
-    requires !a.Nil? && !a.right.Nil?;
-    ensures !b.Nil?;
-    ensures Contents(a) == Contents(b);
-{
-    assume false;
-}
-
-
-// Rotation without color change.
-method WologRotate(direction: Side, a: Node, ghost kc: int) returns (b: Node)
-    requires RBTree(a, kc);
-    requires !a.Nil? && !child(a, opposite(direction)).Nil?;
-    ensures Contents(a) == Contents(b);
-{
-    if direction.Left? {
-        b := RotateLeft(a, kc);
-    } else {
-        b := RotateRight(a, kc);
-    }
-}
+//method RotateRight(a: Node, ghost kc: int) returns (b: Node)
+//    requires RBTree(a, kc);
+//    requires !a.Nil? && !a.left.Nil?;
+//    ensures !b.Nil?;
+//    ensures Contents(a) == Contents(b);
+//{
+//    var l := a.left;
+//    var r := Node(l.right, a.value, a.right, Black);
+//
+//    // Dafny needs help realizing why everything in r is right of l.value;
+//    // it needs me to point out that l.value < a.value.
+//    forall x | x in Contents(r) 
+//        ensures l.value <= x;
+//    {
+//        assert OrderedTree(l);
+//        assert l.value in Contents(a.left);
+//        // Think about the cases, Dafny! (In particular, expand Contents).
+//        if x in Contents(r.left) {
+//        } else if x in Contents(r.right) {
+//        } else if x in multiset{r.value} {
+//        }
+//    }
+//    // A similar property that r.left (l.right) is left of r.value, because
+//    // it was left of a.value in the precondition.
+//    forall x | x in Contents(r.left)
+//        ensures x <= r.value;
+//    {
+//        assert x in Contents(a.left);
+//    }
+//
+//    b := Node(l.left, l.value, r, Black);
+//}
 
 function method redOnRedViolation(tree: Node) : Option<Side>
 {
-    if !ColorOf(tree).Red? then
+    if ColorOf(tree).Black? then
         None
     else if ColorOf(tree.left).Red? then
         Some(Left)
@@ -218,6 +195,7 @@ method RepairCase3Recolor(tree: Node, ghost kc: int, value: int, changedSide: Si
     requires ValueIsOrdered(value, changedSide, tree.value);
     requires MostlyRBTree(child(tree, changedSide), SubtreeBlackCount(tree, kc), value, changedSubtree);
     ensures MostlyRBTree(tree, kc, value, b);
+    ensures Contents(child(b, opposite(changedSide))) == Contents(child(tree, opposite(changedSide)));
 {
     var stableSide := opposite(changedSide);
     var stableSubtree := child(tree, stableSide);
@@ -234,12 +212,18 @@ method RepairCase3Recolor(tree: Node, ghost kc: int, value: int, changedSide: Si
 }
 
 method RepairCase4pt1RotateOutside(childTree: Node, ghost kcc: int, value: int, changedTree: Node, changedSide: Side) returns (rotated: Node)
+    // changedSide is the side of childTree that changed -- the red-on-red
+    // violation child.
     requires RBTree(childTree, kcc);
     requires MostlyRBTree(childTree, kcc, value, changedTree);
-    requires ColorOf(childTree).Red?;
-    requires ColorOf(child(childTree, changedSide)).Red?;
+    //requires ColorOf(childTree).Red?;
+    requires ColorOf(changedTree).Red?;
+    requires ColorOf(child(changedTree, changedSide)).Red?;
     ensures MostlyRBTree(childTree, kcc, value, rotated);
+    ensures ColorOf(rotated).Red?;
+    ensures ColorOf(child(rotated, opposite(changedSide))).Red?;
 {
+/*
     assert ColorOf(childTree).Red?;
     var stableSide := opposite(changedSide);
     var sub1 := child(childTree, stableSide);
@@ -247,9 +231,30 @@ method RepairCase4pt1RotateOutside(childTree: Node, ghost kcc: int, value: int, 
     assert ColorOf(inner).Red?;
     var sub2 := child(inner, stableSide);
     var sub3 := child(inner, changedSide);
+*/
+    var stableSide := opposite(changedSide);
+    var sub1 := child(changedTree, stableSide);
+    var inner := child(changedTree, changedSide);
+    assert ColorOf(inner).Red?;
+    var sub2 := child(inner, stableSide);
+    var sub3 := child(inner, changedSide);
 
-    var outer := WologNode(changedSide, sub1, sub2, changedTree.value, Red);
-    rotated := WologNode(changedSide, outer, sub3, inner.value, Red);
+    var outer := WologNode(stableSide, sub1, sub2, changedTree.value, Red);
+    rotated := WologNode(changedSide, sub3, outer, inner.value, Red);
+
+    // Whoah. Somehow this whole calculation is required to get OrderedTree,
+    // which is bizarre. These spooky actions-at-a-distance make me suspect I'm
+    // bumping into unrolling limits from having recursive definitions opened.
+    // Instant regret.
+    assert Contents(rotated) == Contents(changedTree);  // observe
+    assert Contents(rotated) == Contents(childTree) + multiset{value}; // goal
+
+    assert OrderedTree(inner);  // observe to unpack recursion for sub2
+    assert ValueIsOrdered(inner.value, changedSide, changedTree.value); // observe
+    assert OrderedTree(rotated);  // goal
+
+    assert BlackCountOnAllPaths(inner, kcc);    // observe (recursive unpack)
+//    assert BlackCountOnAllPaths(rotated, kcc);    // goal
 }
 
 lemma BlackCountInheritance(t: Node, kcc: int)
@@ -271,8 +276,6 @@ method RepairCase4pt2RotateUp(tree: Node, ghost kc: int, value:int, changedSide:
     requires SideIsOrdered(changedSubtree, changedSide, tree.value);
     // Stable grandchild didn't change.
     requires child(tree, changedSide).Node?;
-    requires child(changedSubtree, opposite(changedSide))
-        == child(child(tree, changedSide), opposite(changedSide));
     requires MostlyRBTree(child(tree, changedSide), kc - 1, value, changedSubtree);
     ensures MostlyRBTree(tree, kc, value, b);
 {
@@ -303,150 +306,198 @@ method RepairCase4pt2RotateUp(tree: Node, ghost kc: int, value:int, changedSide:
     assert Contents(b) == Contents(changedSubtree) + Contents(uncle) + multiset{tree.value};   // OBSERVE
 }
 
-//XX
-//XXmethod RepairCase2Terminate(tree: Node, ghost kc: int, value: int, changedSide: Side, changedSubtree: Node) returns (b: Node)
-//XX    requires MostlyRBTree(child(tree, changedSide), kc, value, changedSubtree);
-//XX    ensures MostlyRBTree(tree, kc, value, b);
-//XX{
-//XX    var stableSide := opposite(changedSide);
-//XX    var stableSubtree := child(tree, stableSide);
-//XX    b := WologNode(changedSide, changedSubtree, stableSubtree,
-//XX        tree.value, tree.color);
-//XX    assert RedNodesHaveBlackChildren(b.left);
-//XX    assert RedNodesHaveBlackChildren(b.right);
-//XX    assert Contents(b) == Contents(tree) + multiset{value};
-//XX    assert BlackCountOnAllPaths(b, kc);
-//XX    assert redOnRedViolation(b).Some? ==> ColorOf(tree).Red?;
-//XX}
-//XX
-//XX// May violate red-has-black-children rule at top level.
-//XX// This implementation will continue checking as it recurses back up
-//XX// the tree, but that's okay because we have to rebuild the tree pointers
-//XX// anyway.
-//XXmethod InnerInsert(tree: Node, ghost kc: int, value: int) returns (b: Node)
-//XX    requires RBTree(tree, kc);
-//XX    ensures MostlyRBTree(tree, kc, value, b);
-//XX{
-//XX    if tree.Nil? {
-//XX        b := Node(Nil, value, Nil, Red);
-//XX        assert MostlyRBTree(tree, kc, value, b);
-//XX    } else {
-//XX        var changedSide := if (value < tree.value) then Left else Right;
-//XX        var stableSide := opposite(changedSide);
-//XX        ghost var kcc := SubtreeBlackCount(tree, kc);
-//XX        var stableSubtree := child(tree, stableSide);
-//XX        var changedSubtree := InnerInsert(child(tree, changedSide), kcc, value);
-//XX        assert MostlyRBTree(child(tree, changedSide), kcc, value, changedSubtree);
-//XX
-//XX        var violation := redOnRedViolation(changedSubtree);
-//XX        if (violation.Some?) {
-//XX            assert ColorOf(changedSubtree).Red?;
-//XX            if ColorOf(changedSubtree) == ColorOf(stableSubtree) {
-//XX                b := RepairCase3Recolor(tree, kc, value,
-//XX                    changedSide, changedSubtree);
-//XX            }
-//XX
-//XX            var grandchildSide := violation.t;
-//XX            if (grandchildSide != changedSide) {
-//XX                changedSubtree := RepairCase4pt1RotateOutside(child(tree, changedSide), kcc, value, changedSubtree, changedSide);
-//XX                grandchildSide := changedSide;
-//XX            }
-//XX
-//XX            b := RepairCase4pt2RotateUp(tree, kc, value, changedSide, changedSubtree);
-//XX        } else {
-//XX            b := RepairCase2Terminate(tree, kc, value, changedSide, changedSubtree);
-//XX        }
-//XX    }
-//XX}
-//XX
-//XXmethod Insert(tree: Node, ghost kc: int, value: int) returns (updated: Node, ghost ukc: int)
-//XX    requires RBTree(tree, kc);
-//XX    ensures RBTree(updated, ukc);
-//XX    ensures Contents(updated) == Contents(tree) + multiset{value};
-//XX{
-//XX    updated := InnerInsert(tree, kc, value);
-//XX    assert RBTree(updated, ukc);
-//XX    assert Contents(updated) == Contents(tree) + multiset{value};
-//XX}
-//XX
-//XX
-//XX/*
-//XXmethod Contains(tree: Node, value: int) returns (present: bool)
-//XX    requires RBTree(tree);
-//XX    ensures present == (value in Contents(tree));
-//XX{
-//XX    if tree.Nil? {
-//XX        present := false;
-//XX        return;
-//XX    }
-//XX    if value == tree.value {
-//XX        present := true;
-//XX        return;
-//XX    }
-//XX    if value < tree.value {
-//XX        present := Contains(tree.left, value);
-//XX        return;
-//XX    }
-//XX    present := Contains(tree.right, value);
-//XX}
-//XX
-//XX*/
-//XX
-//XXmethod spaces(indent: int) {
-//XX    var i := 0;
-//XX    while (i < indent) {
-//XX        print " ";
-//XX        i := i + 1;
-//XX    }
-//XX}
-//XX
-//XXmethod printTree(t: Node, indent: int) {
-//XX    if (t.Nil?) {
-//XX        return;
-//XX    }
-//XX    printTree(t.left, indent+2);
-//XX    spaces(indent);
-//XX    print t.value;
-//XX    print "\n";
-//XX    printTree(t.right, indent+2);
-//XX}
-//XX
-//XXpredicate eRBTree(tree: Node) {
-//XX    exists kc :: RBTree(tree, kc)
-//XX}
-//XX
-//XXmethod eInsert(tree: Node, value: int) returns (updated: Node)
-//XX    requires eRBTree(tree);
-//XX    ensures eRBTree(updated);
-//XX{
-//XX    ghost var kc :| RBTree(tree, kc);
-//XX    ghost var ekc : int;
-//XX    updated, ekc := Insert(tree, kc, value);
-//XX}
-//XX
-//XXmethod Main() {
-//XX    var t := Nil;
-//XX    RBTreeNil(t);
-//XX    t := eInsert(t, 6);
-//XX    t := eInsert(t, 3);
-//XX    t := eInsert(t, 8);
-//XX    t := eInsert(t, 4);
-//XX    t := eInsert(t, 1);
-//XX    t := eInsert(t, 7);
-//XX    t := eInsert(t, 9);
-//XX    printTree(t, 0);
-//XX    print Contents(t);
-//XX    print "\n";
-//XX
-//XX    t := Nil;
-//XX    t := eInsert(t, 1);
-//XX    t := eInsert(t, 3);
-//XX    t := eInsert(t, 4);
-//XX    t := eInsert(t, 6);
-//XX    t := eInsert(t, 7);
-//XX    t := eInsert(t, 8);
-//XX    t := eInsert(t, 9);
-//XX    printTree(t, 0);
-//XX    print Contents(t);
-//XX    print "\n";
-//XX}
+
+method RepairCase2Terminate(tree: Node, ghost kc: int, value: int, changedSide: Side, changedSubtree: Node) returns (b: Node)
+    requires tree.Node?;
+    requires RBTree(tree, kc);
+    requires redOnRedViolation(changedSubtree).None?;
+    requires MostlyRBTree(child(tree, changedSide), kc, value, changedSubtree);
+    ensures MostlyRBTree(tree, kc, value, b);
+{
+    assume false;   //XXX
+    var stableSide := opposite(changedSide);
+    var stableSubtree := child(tree, stableSide);
+    b := WologNode(changedSide, changedSubtree, stableSubtree,
+        tree.value, tree.color);
+    assert RedNodesHaveBlackChildren(tree);
+    assert RedNodesHaveBlackChildren(stableSubtree);
+    assert RedNodesHaveBlackChildren(changedSubtree);
+    assert Contents(b) == Contents(tree) + multiset{value};
+    assert BlackCountOnAllPaths(changedSubtree, kc - 1);
+    assert BlackCountOnAllPaths(stableSubtree, kc - 1);
+    assert BlackCountOnAllPaths(b, kc);
+    assert redOnRedViolation(b).None?;
+    assert redOnRedViolation(b).Some? ==> ColorOf(tree).Red?;
+    assert OrderedTree(b);
+}
+
+// We don't have this property. Tree rotations break it.
+predicate Stableness(tree: Node, b: Node, changedSide: Side)
+{
+    tree.Node? ==> (
+        b.Node?
+        && Contents(child(b, opposite(changedSide))) == Contents(child(tree, opposite(changedSide)))
+    )
+}
+
+// May violate red-has-black-children rule at top level.
+// This implementation will continue checking as it recurses back up
+// the tree, but that's okay because we have to rebuild the tree pointers
+// anyway.
+method InnerInsert(tree: Node, ghost kc: int, value: int)
+    returns (b: Node, ghost changedSideOut: Side)
+    requires RBTree(tree, kc);
+    ensures MostlyRBTree(tree, kc, value, b);
+    ensures redOnRedViolation(b).Some? ==> ColorOf(child(tree, changedSideOut)).Red?;
+    ensures Stableness(tree, b, changedSideOut);
+{
+    if tree.Nil? {
+        b := Node(Nil, value, Nil, Red);
+        assert MostlyRBTree(tree, kc, value, b);
+        assert Stableness(tree, b, changedSideOut);
+    } else {
+        var changedSide := if (value < tree.value) then Left else Right;
+        var stableSide := opposite(changedSide);
+        ghost var kcc := SubtreeBlackCount(tree, kc);
+        var stableSubtree := child(tree, stableSide);
+        var changedSubtree, insertChanged :=
+            InnerInsert(child(tree, changedSide), kcc, value);
+        assert MostlyRBTree(child(tree, changedSide), kcc, value, changedSubtree);
+
+        var violation := redOnRedViolation(changedSubtree);
+        if (violation.Some?) {
+            assert ColorOf(changedSubtree).Red?;
+            if ColorOf(changedSubtree) == ColorOf(stableSubtree) {
+                b := RepairCase3Recolor(tree, kc, value,
+                    changedSide, changedSubtree);
+                assert (Contents(child(b, opposite(changedSide))) == Contents(child(tree, opposite(changedSide))));
+            } else {
+                assert ColorOf(tree).Black?;
+                    // or else we couldn't have got a red-on-red violation
+                assert ColorOf(changedSubtree).Red?;
+
+                var grandchildSide := violation.t;
+                if (grandchildSide != changedSide) {
+                    var origChild := child(tree, changedSide);
+                    changedSubtree := RepairCase4pt1RotateOutside(origChild, kcc, value, changedSubtree, grandchildSide);
+                    grandchildSide := changedSide;
+
+                    assert ColorOf(child(changedSubtree, changedSide)).Red?;
+//                    assert child(changedSubtree, opposite(changedSide)) == child(origChild, opposite(changedSide));
+//                    assert child(changedSubtree, opposite(changedSide)) == child(child(tree, changedSide), opposite(changedSide));
+                    assert ColorOf(changedSubtree).Red?;
+                }
+
+                assert ColorOf(child(changedSubtree, changedSide)).Red?;
+//                assert child(changedSubtree, opposite(changedSide)) == child(child(tree, changedSide), opposite(changedSide));
+                assert ColorOf(changedSubtree).Red?;
+                b := RepairCase4pt2RotateUp(tree, kc, value, changedSide, changedSubtree);
+                assert (Contents(child(b, opposite(changedSide))) == Contents(child(tree, opposite(changedSide))));
+            }
+            assert (Contents(child(b, opposite(changedSide))) == Contents(child(tree, opposite(changedSide))));
+            assert Stableness(tree, b, changedSide);
+        }
+        else
+        {
+            assert ColorOf(tree).Black?;
+            b := RepairCase2Terminate(tree, kc, value, changedSide, changedSubtree);
+            assert Stableness(tree, b, changedSide);
+        }
+        changedSideOut := changedSide;
+        assert Stableness(tree, b, changedSideOut);
+    }
+    assert Stableness(tree, b, changedSideOut);
+}
+
+method Insert(tree: Node, ghost kc: int, value: int) returns (updated: Node, ghost ukc: int)
+    requires RBTree(tree, kc);
+    ensures RBTree(updated, ukc);
+    ensures Contents(updated) == Contents(tree) + multiset{value};
+{
+    ghost var innerChanged: Side;
+    updated, innerChanged := InnerInsert(tree, kc, value);
+    assert RBTree(updated, ukc);
+    assert Contents(updated) == Contents(tree) + multiset{value};
+}
+
+
+/*
+method Contains(tree: Node, value: int) returns (present: bool)
+    requires RBTree(tree);
+    ensures present == (value in Contents(tree));
+{
+    if tree.Nil? {
+        present := false;
+        return;
+    }
+    if value == tree.value {
+        present := true;
+        return;
+    }
+    if value < tree.value {
+        present := Contains(tree.left, value);
+        return;
+    }
+    present := Contains(tree.right, value);
+}
+
+*/
+
+method spaces(indent: int) {
+    var i := 0;
+    while (i < indent) {
+        print " ";
+        i := i + 1;
+    }
+}
+
+method printTree(t: Node, indent: int) {
+    if (t.Nil?) {
+        return;
+    }
+    printTree(t.left, indent+2);
+    spaces(indent);
+    print t.value;
+    print "\n";
+    printTree(t.right, indent+2);
+}
+
+predicate eRBTree(tree: Node) {
+    exists kc :: RBTree(tree, kc)
+}
+
+method eInsert(tree: Node, value: int) returns (updated: Node)
+    requires eRBTree(tree);
+    ensures eRBTree(updated);
+{
+    ghost var kc :| RBTree(tree, kc);
+    ghost var ekc : int;
+    updated, ekc := Insert(tree, kc, value);
+}
+
+method Main() {
+    var t := Nil;
+    RBTreeNil(t);
+    t := eInsert(t, 6);
+    t := eInsert(t, 3);
+    t := eInsert(t, 8);
+    t := eInsert(t, 4);
+    t := eInsert(t, 1);
+    t := eInsert(t, 7);
+    t := eInsert(t, 9);
+    printTree(t, 0);
+    print Contents(t);
+    print "\n";
+
+    t := Nil;
+    t := eInsert(t, 1);
+    t := eInsert(t, 3);
+    t := eInsert(t, 4);
+    t := eInsert(t, 6);
+    t := eInsert(t, 7);
+    t := eInsert(t, 8);
+    t := eInsert(t, 9);
+    printTree(t, 0);
+    print Contents(t);
+    print "\n";
+}
